LeanMenhir.lean
@@ -10,6 +10,7 @@ import LeanMenhir.Validator.Complete
 import LeanMenhir.Interpreter
 import LeanMenhir.Interpreter.Correct
 import LeanMenhir.Interpreter.Complete
+import LeanMenhir.Interpreter.Congr
 import LeanMenhir.Main
 import LeanMenhir.Runtime
 import LeanMenhir.Generator.FinAlphabet
